src/named/MultiCompilers.v
@@ -21,15 +21,7 @@ Proof.
   reflexivity.
 Qed.
 
-Lemma compile_ctx_empty cmp
-  : compile_ctx cmp [] = [].
-Proof.
-  unfold compile_ctx.
-  rewrite flat_map_all_empty; auto.
-Qed.  
-Hint Rewrite compile_ctx_empty : lang_core.
-
-
+(*
 Lemma map_flat_map {A B C} (f : B -> C) (g : A -> list B) l
   : map f (flat_map g l) = flat_map (fun x => map f (g x)) l.
 Admitted.
@@ -105,7 +97,7 @@ Proof.
     cbv [compile_ctx fst named_map].
     simpl.
     unfold In.*)
-Admitted.
+Admitted.*)
 (*
 Hint Rewrite fresh_compile_ctx : lang_core.*)
 
@@ -154,11 +146,11 @@ Proof.
   rewrite H, IHl; auto.
 Qed.
 
-Lemma compile_strengthen_term cmp n cc e cname
-  : fresh n (snd cmp) ->
-    all_fresh (snd cmp) ->
-    all_constructors (fun n => In n (map fst (snd cmp))) e ->
-    compile (extend_cmp [(n,cc)] cmp) cname e = compile cmp cname e.
+Lemma compile_strengthen_term cnames ccs n cc e cname
+  : fresh n ccs ->
+    all_fresh ccs ->
+    all_constructors (fun n => In n (map fst ccs)) e ->
+    compile (cnames,(n,cc)::ccs) cname e = compile (cnames,ccs) cname e.
 Proof.
   revert cname.
   induction e; basic_goal_prep; basic_core_crush.
@@ -170,14 +162,10 @@ Proof.
     basic_core_crush.
   f_equal.
   f_equal.
-  apply flat_map_funext.
-  intros x Inx.
-  apply map_ext_in.
-  intros a Ina.
-  pose proof (in_all _ _ H Ina).
-  simpl in *.
-  apply H2; auto.
-  eapply in_all; eauto.
+  apply flat_map_funext; intros.
+  apply map_ext_in; intros.
+  eapply in_all in H; eauto.
+  eapply in_all in H4; eauto.
 Qed.
 Hint Rewrite compile_strengthen_term : lang_core.
 
@@ -187,66 +175,58 @@ Lemma compile_args_cons_eq l n1 n2 a e
     compile_args (l, n1) e = compile_args (l, n2) e ->
     compile_args (l, n1) (a :: e) = compile_args (l, n2) (a :: e).
 Proof.
-  unfold compile_args.
-  induction l; basic_goal_prep; basic_core_crush.
+  simpl.
+  intros Ha ->.
   f_equal.
-  {
-    clear IHl.
-    append_eq_same_len
+  eauto using map_ext_in.
 Qed.
 
-Lemma compile_strengthen_args cmp n cc e
-  : fresh n (snd cmp) ->
-    all_fresh (snd cmp) ->
-    all (all_constructors (fun n => In n (map fst (snd cmp)))) e ->
-    compile_args (extend_cmp [(n,cc)] cmp) e = compile_args cmp e.
+Lemma compile_strengthen_args cnames ccs n cc e
+  : fresh n ccs ->
+    all_fresh ccs ->
+    all (all_constructors (fun n => In n (map fst ccs))) e ->
+    compile_args (cnames, (n,cc)::ccs) e = compile_args (cnames, ccs) e.
 Proof.
   induction e; basic_goal_prep; basic_core_crush.
-  apply compile_args_cons_eq.
-  basic_goal_prep; basic_core_crush.
-  unfold compile_args.
-  simpl.
+  apply compile_args_cons_eq;
+    basic_goal_prep; basic_core_crush.
 Qed.
 Hint Rewrite compile_strengthen_args : lang_core.
 
-Lemma compile_strengthen_sort cmp n cc e
-  : fresh n cmp ->
-    all_fresh cmp ->
-    all_constructors_sort (fun n => In n (map fst cmp)) e ->
-    compile_sort ((n,cc)::cmp) e = compile_sort cmp e.
+Lemma compile_strengthen_sort cnames ccs n cc e cname
+  : fresh n ccs ->
+    all_fresh ccs ->
+    all_constructors_sort (fun n => In n (map fst ccs)) e ->
+    compile_sort (cnames,(n,cc)::ccs) cname e = compile_sort (cnames, ccs) cname e.
 Proof.
   destruct e; basic_goal_prep; basic_core_crush.
-  my_case Heq (eqb v n); basic_goal_prep;
+  my_case Heq (eqb l n); basic_goal_prep;
     basic_core_crush.
-  case_match; basic_goal_prep;
-      basic_core_crush.
-  case_match; basic_goal_prep;
-    basic_core_crush.
-  f_equal.
-  f_equal.
-  apply compile_strengthen_args; assumption.
 Qed.
 Hint Rewrite compile_strengthen_sort : lang_core.
 
 
-Lemma compile_strengthen_ctx cmp n cc c
-  : fresh n cmp ->
-    all_fresh cmp ->
-    all (fun '(_,t) => all_constructors_sort (fun n => In n (map fst cmp)) t) c ->
-    compile_ctx ((n,cc)::cmp) c = compile_ctx cmp c.
+Lemma compile_strengthen_ctx cnames ccs n cc c
+  : fresh n ccs ->
+    all_fresh ccs ->
+    all (fun '(_,t) => all_constructors_sort (fun n => In n (map fst ccs)) t) c ->
+    compile_ctx (cnames,(n,cc)::ccs) c = compile_ctx (cnames, ccs) c.
 Proof.
   induction c; basic_goal_prep; f_equal; basic_core_crush.
+  apply map_ext_in; intros; f_equal.
+  basic_core_crush.
 Qed.
 Hint Rewrite compile_strengthen_ctx : lang_core.
 
 
-Lemma sort_name_in_cmp cmp_pre tgt cmp src c' args n
-  : preserving_compiler_ext cmp_pre tgt cmp src ->
+Lemma sort_name_in_cmp cmp_pre tgt ccs src c' args n
+  : preserving_compiler_ext cmp_pre tgt ccs src ->
     In (n, sort_rule c' args) src ->
-    In n (map fst cmp).
+    In n (map fst ccs).
 Proof.
   induction 1;basic_goal_prep;
     with_rule_in_wf_crush.
+  all: try typeclasses eauto. (*TODO: put in with_rule_if_wf_crush*)
 Qed.
 Local Hint Resolve sort_name_in_cmp : lang_core.
 
@@ -257,41 +237,43 @@ Lemma term_name_in_cmp cmp_pre tgt cmp src c' args t n
 Proof.
   induction 1;basic_goal_prep;
     with_rule_in_wf_crush.
+  all: try typeclasses eauto. (*TODO: put in with_rule_if_wf_crush*)
 Qed.
 Local Hint Resolve term_name_in_cmp : lang_core.
                    
-Local Lemma all_constructors_from_wf tgt cmp src
-  : preserving_compiler_ext [] tgt cmp src ->
+Local Lemma all_constructors_from_wf cnames tgt cmp src
+  : preserving_compiler_ext (cnames,[]) tgt cmp src ->
     (forall c t,
         wf_sort src c t ->
-        all_constructors_sort (fun n0 : V => In n0 (map fst cmp)) t)
+        all_constructors_sort (fun n0 => In n0 (map fst cmp)) t)
     /\ (forall c e t,
            wf_term src c e t ->
-           all_constructors (fun n0 : V => In n0 (map fst cmp)) e)
+           all_constructors (fun n0 => In n0 (map fst cmp)) e)
     /\ (forall c s c',
            wf_args src c s c' ->
-           all (all_constructors (fun n0 : V => In n0 (map fst cmp))) s).
+           all (all_constructors (fun n0 => In n0 (map fst cmp))) s).
 Proof using.
   intros; apply wf_judge_ind; basic_goal_prep;
     with_rule_in_wf_crush.
+  all: try typeclasses eauto. (*TODO: put in with_rule_if_wf_crush*)
 Qed.
 
-Definition all_constructors_sort_from_wf tgt cmp src (pr : preserving_compiler_ext [] tgt cmp src)
+Definition all_constructors_sort_from_wf cnames tgt cmp src (pr : preserving_compiler_ext (cnames,[]) tgt cmp src)
   := proj1 (all_constructors_from_wf pr).
 Hint Resolve all_constructors_sort_from_wf : lang_core.
 
-Definition all_constructors_term_from_wf tgt cmp src (pr : preserving_compiler_ext [] tgt cmp src)
+Definition all_constructors_term_from_wf cnames tgt cmp src (pr : preserving_compiler_ext (cnames,[]) tgt cmp src)
   := proj1 (proj2 (all_constructors_from_wf pr)).
 Hint Resolve all_constructors_term_from_wf : lang_core.
 
-Definition all_constructors_args_from_wf tgt cmp src (pr : preserving_compiler_ext [] tgt cmp src)
+Definition all_constructors_args_from_wf cnames tgt cmp src (pr : preserving_compiler_ext (cnames,[]) tgt cmp src)
   := proj2 (proj2 (all_constructors_from_wf pr)).
 Hint Resolve all_constructors_args_from_wf : lang_core.
 
-Lemma all_constructors_ctx_from_wf tgt cmp src c
-  : preserving_compiler_ext [] tgt cmp src ->
+Lemma all_constructors_ctx_from_wf cnames tgt cmp src c
+  : preserving_compiler_ext (cnames,[]) tgt cmp src ->
     wf_ctx src c ->
-    all_constructors_ctx (fun n0 : V => In n0 (map fst cmp)) c.
+    all_constructors_ctx (fun n0 => In n0 (map fst cmp)) c.
 Proof.
   induction 2; basic_goal_prep;
     with_rule_in_wf_crush.
@@ -299,36 +281,47 @@ Qed.
 Hint Resolve all_constructors_ctx_from_wf : lang_core.
 
 
+  (*TODO: lift*)
+Ltac use_in_all :=
+  repeat lazymatch goal with
+  | [H : all _ _|-_] =>
+      simple eapply in_all in H; [|eassumption]
+  end.
+
 (*TODO: think about whether this should be generalized*)
-Lemma inductive_implies_semantic_sort_axiom ls lt cmp name c t1 t2
-  : wf_lang lt -> preserving_compiler_ext [] lt cmp ls -> wf_lang ls ->
+Lemma inductive_implies_semantic_sort_axiom cnames ls lt cmp name c t1 t2 cname
+  : wf_lang lt -> preserving_compiler_ext (cnames,[]) lt cmp ls -> wf_lang ls ->
+    In cname cnames ->
     In (name, sort_eq_rule c t1 t2) ls ->
-    eq_sort lt (compile_ctx cmp c) (compile_sort cmp t1) (compile_sort cmp t2).
+    eq_sort lt (compile_ctx (cnames,cmp) c) (compile_sort (cnames,cmp) cname t1) (compile_sort (cnames,cmp) cname t2).
 Proof.
   induction 2;
-    basic_goal_prep; try use_rule_in_wf;
+    basic_goal_prep; try use_rule_in_wf; use_in_all;
       basic_core_firstorder_crush.
-  (*TODO: why is this needed? should be automated*)
+  (*TODO: why is this needed? should be automated*)  
   all: use_rule_in_wf;autorewrite with lang_core utils in *;
     intuition eauto with lang_core.
 Qed.
 
 
-Lemma inductive_implies_semantic_term_axiom ls lt cmp name c e1 e2 t
-  : wf_lang lt -> preserving_compiler_ext [] lt cmp ls -> wf_lang ls ->
+Lemma inductive_implies_semantic_term_axiom cnames ls lt cmp name c e1 e2 t cname
+  : wf_lang lt -> preserving_compiler_ext (cnames,[]) lt cmp ls -> wf_lang ls ->
+    In cname cnames ->
     In (name, term_eq_rule c e1 e2 t) ls ->
-    eq_term lt (compile_ctx cmp c) (compile_sort cmp t) (compile cmp e1) (compile cmp e2).
+    eq_term lt (compile_ctx (cnames,cmp) c) (compile_sort (cnames,cmp) cname t)
+            (compile (cnames,cmp) cname e1) (compile (cnames,cmp) cname e2).
 Proof.
   induction 2;
     basic_goal_prep;
     try use_rule_in_wf;
+    use_in_all;
     basic_core_firstorder_crush.
   (*TODO: why is this needed? should be automated*)
   all: use_rule_in_wf;autorewrite with lang_core utils in *;
     intuition eauto with lang_core.
 Qed.
 
-
+(*TODO: generalize
 Lemma with_names_from_compile_ctx (A:Type) cmp c (s : list A)
   : with_names_from (compile_ctx cmp c) s
     = with_names_from c s.
@@ -338,12 +331,12 @@ Proof.
   cbn.
   f_equal; basic_core_crush.
 Qed.
-  
+  *)
 
 
-
-Lemma compile_id_args A cmp (c : named_list A)
-  : map (compile cmp) (id_args c) = id_args c.
+(* TODO: generalize*)
+(*Lemma compile_id_args A cmp (c : named_list A)
+  : map (compile mp) (id_args c) = id_args c.
 Proof.
   unfold id_args.
   induction c; 
@@ -351,6 +344,7 @@ Proof.
     basic_core_crush.
 Qed.
 Hint Rewrite compile_id_args : lang_core.
+*)
 
 Lemma fst_equal_id_args_equal A B (c1 : named_list A) (c2 : named_list B)
   : map fst c1 = map fst c2 -> id_args c1 = id_args c2.
@@ -358,109 +352,119 @@ Proof.
   unfold id_args; basic_core_crush.
 Qed.
 
+(*TODO: generalize*)
+(*
 Lemma compile_ctx_fst_equal cmp c
   : map fst (compile_ctx cmp c) = map fst c.
 Proof.
   induction c; break; simpl; f_equal; auto.
 Qed.
- 
-
-Lemma inductive_implies_semantic_sort_rule_id ls lt cmp name c args
-  : wf_lang lt -> preserving_compiler_ext [] lt cmp ls -> wf_lang ls ->
-    In (name, sort_rule c args) ls ->
-    wf_sort lt (compile_ctx cmp c) (compile_sort cmp (scon name (id_args c))).
-Proof.
-  intros wfl pr wfl';
-    revert wfl'; induction pr;
-      basic_goal_prep;
-      with_rule_in_wf_crush.
-  all: try eapply all_constructors_ctx_from_wf; eauto with lang_core.
-  {
-    my_case Hname (eqb name n);[|case_match]; basic_core_firstorder_crush.
-  }
-  {
-    use_rule_in_wf; basic_core_crush.
-  }
-  {
-    my_case Hname (eqb name n);[|case_match]; basic_core_crush.
-  }
-  4:{
-    use_rule_in_wf; basic_core_crush.
-  }
-  (*TODO: eqb? where did this come from?*)
-  all: constructor.
-Qed.
-
-
-
-Lemma inductive_implies_semantic_term_rule_id ls lt cmp name c args t
-  : wf_lang lt -> preserving_compiler_ext [] lt cmp ls -> wf_lang ls ->
-    In (name, term_rule c args t) ls ->
-    wf_term lt (compile_ctx cmp c) (compile cmp (con name (id_args c))) (compile_sort cmp t).
-Proof.
-  intros wfl pr wfl';
-    revert wfl'; induction pr;
-      basic_goal_prep;
-      try use_rule_in_wf;
-      basic_core_firstorder_crush.
-  all: try solve [use_rule_in_wf; basic_core_crush].
-  {
-    my_case Hname (eqb name n);[|case_match]; basic_core_crush.
-  }
-  {
-    my_case Hname (eqb name n);[|case_match]; basic_core_crush.
-  }
-Qed.
-
-
-
-Lemma lookup_in_dom s n
-  : In n (map fst s) -> In (subst_lookup s n) (map snd s).
-Proof.
-  induction s;
-    basic_goal_prep;
-    basic_core_crush.
-  case_match; basic_core_crush.
-Qed.
-
-(*
-Lemma wf_con_id_args_subst' A (c : named_list A) s
-  : forall n e, In n (map fst c) ->
-                In n (map fst s) ->
-                In e (id_args c)[/s/] -> In e (map snd s).
-Proof.
-  induction c;
-    basic_goal_prep;
-    basic_core_crush.
-  (apply lookup_in_dom; assumption).
-  
-  
-  rewrite IHc.
-  unfold args_subst.
 *)
 
-
-Lemma compile_subst_lookup cmp s n
-  : compile cmp (subst_lookup s n)
-  = subst_lookup (compile_subst cmp s) n.
+(*TODO: should be in Utils.v*)
+Lemma named_list_lookup_err_is_Some {A} d l n (v:A)  
+  : Some v = named_list_lookup_err l n ->
+    named_list_lookup d l n = v.
 Proof.
-  induction s;
-    basic_goal_prep;
-    basic_core_crush.
-  case_match; basic_core_crush.
+  induction l; basic_goal_prep.
+  basic_utils_crush.
+  my_case Heq (eqb n s).
+  inversion H; tauto.
+  basic_utils_crush.
 Qed.
-Hint Rewrite compile_subst_lookup : lang_core.
 
 
-Lemma combine_subst args l s
-  : (combine args l)[/s/] = combine args l[/s/].
+Lemma combine_app_same_len {A B} (a1 b1 : list A) (a2 b2 : list B)
+  : length a1 = length a2 ->
+    combine (a1++b1) (a2++b2) = (combine a1 a2) ++ (combine b1 b2).
 Proof.
-  revert args.
-  induction l;
-    destruct args;
-    basic_goal_prep;
-    basic_core_crush.
+  revert a2; induction a1; destruct a2; basic_goal_prep;
+    basic_utils_crush.
 Qed.
+(*Note: not completely safe, but usually useful *)
+Hint Rewrite @combine_app_same_len : utils.
+
+Lemma id_args_app (a b : ctx)
+  : id_args (a++b) = id_args a ++ id_args b.
+Proof.
+  induction a; basic_goal_prep; basic_core_crush.
+Qed.
+Hint Rewrite id_args_app : utils.
+
+Lemma with_names_from_app_same_len {A B} (a1 b1 : named_list A) (a2 b2 : list B)
+  : length a1 = length a2 ->
+    with_names_from (a1++b1) (a2++b2) = (with_names_from a1 a2) ++ (with_names_from b1 b2).
+Proof.
+  revert a2; induction a1; destruct a2; basic_goal_prep;
+    basic_utils_crush.
+Qed.
+(*Note: not completely safe, but usually useful *)
+Hint Rewrite @with_names_from_app_same_len : utils.
+
+
+(*TODO: get rid of with_names_from, or define in terms of combine? *)
+
+(*cmp1,2 an artifact of env_args taking a full compiler*)
+Lemma compile_id_subst cnames cmp1 cmp2 c
+  : combine (env_args (cnames, cmp1) (map fst c))
+            (compile_args (cnames, cmp2) (id_args c))
+    = id_subst (compile_ctx (cnames, cmp2) c).
+Proof.
+  induction c; basic_goal_prep; basic_core_crush.
+  f_equal; eauto.
+  rewrite <- combine_map_fst_is_with_names_from.
+  f_equal;
+    unfold id_args;
+    rewrite !map_map;
+    apply map_ext;
+    basic_goal_prep; basic_core_crush.
+  all: constructor. (*TODO: where does this come from?*)
+Qed.
+
+
+Lemma P_of_named_list_lookup_from_all {A B P} `{Eqb A} (l1 : list A) (l2:list B) n d
+  : all P l2 ->
+    In n l1 ->
+    length l2 = length l1 ->
+    P (named_list_lookup d (combine l1 l2) n).
+Proof.
+  revert l2; induction l1; destruct l2;
+    basic_goal_prep; basic_utils_crush.
+  my_case Heqb (eqb n a);
+    basic_goal_prep; basic_utils_crush.
+Qed.
+
+Lemma P_of_named_list_lookup_from_all_combined {A B P} `{Eqb A} (l1 : list A) (l2:list B) n d
+  : all P (combine l1 l2) ->
+    In n l1 ->
+    length l2 = length l1 ->
+    P (n, (named_list_lookup d (combine l1 l2) n)).
+Proof.
+  revert l2; induction l1; destruct l2;
+    basic_goal_prep; basic_utils_crush.
+  my_case Heqb (eqb n a);
+    basic_goal_prep; basic_utils_crush.
+Qed.
+
+(*TODO: move to utils*)
+Hint Resolve incl_nil_l : utils.
+Hint Resolve incl_tl : utils.
+
+Lemma map_snd_combine_incl {A B} (a : list A) (b : list B)
+  : incl (map snd (combine a b)) b.
+Proof.
+  revert b; induction a; destruct b;
+    basic_goal_prep; basic_utils_crush.
+Qed.  
+
+Lemma all_weaken_incl {A P} (a b : list A)
+  : incl a b -> all P b -> all P a.
+Proof.
+  revert b; induction a;
+    basic_goal_prep; basic_utils_crush.
+  eapply in_all; eauto.
+Qed.
+
 
 
 Lemma lang_compiler_sort_case_args_eq cmp_pre lt cmp ls n c args args' e
@@ -498,139 +502,537 @@ Proof.
 Qed.
 Hint Resolve lang_compiler_term_case_args_eq : lang_core.
 
+Lemma inductive_implies_semantic_sort_rule_id cnames ls lt cmp name c args cname
+  : wf_lang lt -> preserving_compiler_ext (cnames,[]) lt cmp ls -> wf_lang ls ->
+    In (name, sort_rule c args) ls ->
+    In cname cnames ->
+    wf_sort lt (compile_ctx (cnames,cmp) c) (compile_sort (cnames,cmp) cname (scon name (id_args c))).
+Proof.
+  intros wfl pr wfl';
+    revert wfl'; induction pr;
+    basic_goal_prep;
+    use_in_all;
+      with_rule_in_wf_crush.
+  all: try typeclasses eauto.
+  (*TODO: no longer does anything*)
+  all: try eapply all_constructors_ctx_from_wf; eauto with lang_core.
+3:{
+  with_rule_in_wf_crush.
+}
+4:{
+  with_rule_in_wf_crush.
+}
+{
+  rewrite compile_id_subst.
+  rewrite subst_id.
+  simple eapply P_of_named_list_lookup_from_all; eassumption.
+}
+{
+      with_rule_in_wf_crush.
+    my_case Hname (eqb name n);[|case_match]; basic_core_firstorder_crush.
+}
+{
+  my_case Hname (eqb name n);[|case_match]; basic_core_crush.
+}
+Qed.
+
+
+
+Lemma inductive_implies_semantic_term_rule_id cnames ls lt cmp name c args t cname
+  : wf_lang lt -> preserving_compiler_ext (cnames,[]) lt cmp ls -> wf_lang ls ->
+    In (name, term_rule c args t) ls ->
+    In cname cnames ->
+    wf_term lt (compile_ctx (cnames,cmp) c)
+            (compile (cnames,cmp) cname (con name (id_args c)))
+            (compile_sort (cnames,cmp) cname t).
+Proof.
+  intros wfl pr wfl';
+    revert wfl'; induction pr;
+    basic_goal_prep;
+    use_in_all;
+      try use_rule_in_wf;
+      basic_core_firstorder_crush.
+  all: try solve [use_rule_in_wf; basic_core_crush].
+  2:{
+    change (flat_map
+           (fun x : term =>
+            map
+              (fun cname0 : string =>
+                 compile (cnames, ?cmp) cname0 x) cnames))
+    with (compile_args (cnames, cmp)).
+    rewrite compile_id_subst.
+    rewrite subst_id.
+    lazymatch goal with
+      H : all ?P (combine _ _) |- _ =>        
+        eapply (P_of_named_list_lookup_from_all_combined _ _ _ _ H)
+    end; auto.
+  }
+  {
+    my_case Hname (eqb name n);[|case_match]; basic_core_crush.
+    revert H7; case_match; auto.
+    change (flat_map
+           (fun x : term =>
+            map
+              (fun cname0 : string =>
+                 compile (cnames, ?cmp) cname0 x) cnames))
+      with (compile_args (cnames, cmp)).
+    replace args1 with (map fst c).
+    rewrite !compile_id_subst.
+    rewrite !subst_id.
+    auto.
+    symmetry.
+    eapply lang_compiler_term_case_args_eq; try eassumption.
+    basic_core_crush.
+  }
+  {
+    my_case Hname (eqb name n);[|case_match]; basic_core_firstorder_crush.
+    revert H8; case_match; auto.
+    pose proof (lang_compiler_term_case_args_eq _ _ _ _ _ _ pr ltac:(basic_core_crush) H3 HeqH9).
+    subst.
+    all:change (flat_map
+           (fun x : term =>
+            map
+              (fun cname0 : string =>
+                 compile (cnames, ?cmp) cname0 x) cnames))
+      with (compile_args (cnames, cmp)).
+    rewrite !compile_id_subst.
+    rewrite !subst_id.
+    auto.
+  }
+Qed.
+
+
+
+Lemma lookup_in_dom s n
+  : In n (map fst s) -> In (subst_lookup s n) (map snd s).
+Proof.
+  induction s;
+    basic_goal_prep;
+    basic_core_crush.
+  case_match; basic_core_crush.
+Qed.
+
+(*
+Lemma wf_con_id_args_subst' A (c : named_list A) s
+  : forall n e, In n (map fst c) ->
+                In n (map fst s) ->
+                In e (id_args c)[/s/] -> In e (map snd s).
+Proof.
+  induction c;
+    basic_goal_prep;
+    basic_core_crush.
+  (apply lookup_in_dom; assumption).
+  
+  
+  rewrite IHc.
+  unfold args_subst.
+*)
+
+(*TODO: put in utils*)
+Lemma named_list_lookup_notin_app {A B} `{Eqb A} (n : A) l1 l2 (d : B)
+  : ~ In n (map fst l1) ->
+    named_list_lookup d (l1++l2) n = named_list_lookup d l2 n.
+Proof.
+  induction l1;
+    basic_goal_prep;
+    basic_utils_crush.
+  case_match; basic_utils_crush.
+Qed.
+
+(*TODO: put in utils*)
+Lemma named_list_lookup_in_app {A B} `{Eqb A} (n : A) l1 l2 (d : B)
+  : In n (map fst l1) ->
+    named_list_lookup d (l1++l2) n = named_list_lookup d l1 n.
+Proof.
+  induction l1;
+    basic_goal_prep;
+    basic_utils_crush.
+  case_match; basic_utils_crush.
+Qed.
+
+(*TODO: put in utils *)
+Lemma all2_refl {A} `{Eqb A} (l : list A) : all2 eqb l l = true.
+Proof.
+  induction l;
+    basic_goal_prep;
+    basic_utils_crush.
+Qed.
+Hint Rewrite all2_refl : utils.
+
+(*TODO: put in utils *)
+Lemma and_true_l b : (true && b = b)%bool.
+Proof.
+  basic_goal_prep;
+    basic_utils_crush.
+Qed.
+Hint Rewrite and_true_l : utils.
+
+(*TODO: put in utils *)
+Lemma and_true_r b : (b && true = b)%bool.
+Proof.
+  destruct b;
+  basic_goal_prep;
+    basic_utils_crush.
+Qed.
+Hint Rewrite and_true_r : utils.
+
+Lemma compile_subst_lookup cmp s n cname
+  : In cname (fst cmp) ->
+    compile cmp cname (subst_lookup s n)
+  = subst_lookup (compile_subst cmp s) (cname::n).
+Proof.
+  induction s;
+    basic_goal_prep;
+    basic_core_crush.
+  case_match; basic_core_crush.
+  2:{
+    unfold subst_lookup in *.
+    rewrite H0.
+    rewrite named_list_lookup_notin_app; auto.
+    assert (l<> n) by basic_utils_crush.
+    rewrite map_map.
+    simpl.
+    revert H1; clear.
+    induction l0;
+      basic_goal_prep;
+      basic_utils_crush.
+  }
+  {
+    unfold subst_lookup in *.
+    rewrite named_list_lookup_in_app; simpl; auto.
+    2:{
+      rewrite map_map; simpl.
+      revert H; clear.
+      induction l0;
+      basic_goal_prep;
+      basic_utils_crush.
+    }
+    
+    revert H; clear.
+    generalize (compile (l0,n0)) as cf; intro.
+    induction l0;
+      basic_goal_prep;
+      basic_utils_crush.
+    case_match;
+      basic_goal_prep;
+      basic_utils_crush.
+  }
+Qed.
+Hint Rewrite compile_subst_lookup : lang_core.
+
+
+Lemma combine_subst args l s
+  : (combine args l)[/s/] = combine args l[/s/].
+Proof.
+  revert args.
+  induction l;
+    destruct args;
+    basic_goal_prep;
+    basic_core_crush.
+Qed.
+
+(*TODO: move to utils*)
+Hint Rewrite map_map : utils.
+Hint Rewrite map_app : utils.
+
+Lemma env_args_as_fst_ctx cmp1 cmp2 c
+  : fst cmp1 = fst cmp2 ->
+    (env_args cmp1 (map fst c))
+    = (map fst (compile_ctx cmp2 c)).
+Proof.
+  induction c; basic_goal_prep; basic_core_firstorder_crush.
+Qed.
+
+Lemma all_impl {A} {P Q : _ -> Prop} (l : list A)
+  : (forall a, In a l -> P a -> Q a) -> all P l -> all Q l.
+Proof.
+  intro; induction l; basic_goal_prep; basic_utils_crush.
+Qed.
 
 Lemma sort_case_in_preserving_well_scoped cmp_pre tgt cmp src n args t
   : preserving_compiler_ext cmp_pre tgt cmp src ->
     ws_lang tgt ->
     In (n, sort_case args t) cmp ->
-    well_scoped args t.
+    all (well_scoped (env_args cmp_pre args)) t.
 Proof.
   induction 1; basic_goal_prep; basic_core_firstorder_crush.
-  erewrite <- compile_ctx_fst_equal.
-  eapply wf_sort_implies_ws; eauto; eauto with term lang_core.
+  erewrite env_args_as_fst_ctx.
+  eapply all_impl; [|eassumption].
+  basic_goal_prep; basic_core_firstorder_crush.
+  destruct cmp_pre; reflexivity.
 Qed.
 Hint Resolve sort_case_in_preserving_well_scoped : lang_core.
 
+(*TODO: move to utils*)
+Tactic Notation "open_generalize" uconstr(c) :=
+  let a' := fresh "v" in
+  let a := fresh "v" in
+  set c as a; generalize a as a'; clear a.
 
 Lemma term_case_in_preserving_well_scoped cmp_pre tgt cmp src n args t
   : preserving_compiler_ext cmp_pre tgt cmp src ->
     ws_lang tgt ->
     In (n, term_case args t) cmp ->
-    well_scoped args t.
+    well_scoped (env_args cmp_pre args) t.
 Proof.
   induction 1; basic_goal_prep; basic_core_firstorder_crush.
-  erewrite <- compile_ctx_fst_equal.
-  eapply wf_term_implies_ws; eauto; eauto with term lang_core.
+  assert (all (fun p => well_scoped (env_args cmp_pre (map fst c)) (snd p))
+              (combine (fst cmp_pre) t)).
+  {
+    erewrite env_args_as_fst_ctx.
+    eapply all_impl; [|eassumption].
+    basic_goal_prep.
+    basic_core_firstorder_crush.
+    destruct cmp_pre; reflexivity.
+  }
+  destruct cmp_pre; simpl in *;
+    revert H4 H1; clear.
+  open_generalize (env_args _ _); intro args.
+  revert l0; induction t; destruct l0; 
+    basic_goal_prep;
+    basic_core_firstorder_crush.
 Qed.
 Hint Resolve term_case_in_preserving_well_scoped : lang_core.
 
-(*TODO: move to term?
-  TODO: make type inference smoother
-*)
-Lemma subst_term_default s
-  : (@default term (@term_default V _) : term)[/s/]
-    = (@default term (@term_default V _) : term).
+
+(*cmp1,2 an artifact of env_args taking a full compiler*)
+Lemma compile_args_to_subst {B} cnames cmp1 cmp2 c (l : list B)
+  : combine (env_args (cnames, cmp1) (map fst c)) l
+    = with_names_from (compile_ctx (cnames, cmp2) c) l.
 Proof.
-  unfold default.
-  unfold term_default.
-  simpl.
-  reflexivity.
+  induction c; basic_goal_prep; basic_core_crush.
+  rewrite <- combine_map_fst_is_with_names_from.
+  basic_core_crush.
+  f_equal.
+  f_equal.
+  apply env_args_as_fst_ctx; auto.
 Qed.
 
-Local Lemma distribute_compile_subst tgt cmp src s
-  : preserving_compiler_ext [] tgt cmp src ->
+
+Lemma sort_case_length_in_preserving cnames cmp_pre tgt cmp src n args t
+  : preserving_compiler_ext (cnames, cmp_pre) tgt cmp src ->
+    In (n, sort_case args t) cmp ->
+    length t = length cnames.
+Proof.
+  induction 1; basic_goal_prep; basic_core_crush.
+Qed.
+
+
+Lemma term_case_length_in_preserving cnames cmp_pre tgt cmp src n args t
+  : preserving_compiler_ext (cnames, cmp_pre) tgt cmp src ->
+    In (n, term_case args t) cmp ->
+    length t = length cnames.
+Proof.
+  induction 1; basic_goal_prep; basic_core_crush.
+Qed.
+
+
+
+
+Require Import Lia.
+(*TODO: move to utils*)
+Hint Rewrite app_length : utils.
+Lemma flat_map_const_len {A B} (f : A -> list B) len l
+  : (forall a, length (f a) = len) ->
+    length (flat_map f l) = len * length l.
+Proof.
+  intros; induction l;
+    basic_goal_prep;
+    basic_utils_crush.
+  simpl.
+  specialize (H a).
+  lia.
+Qed.
+
+Local Lemma distribute_compile_subst cnames tgt cmp src s
+  : preserving_compiler_ext (cnames,[]) tgt cmp src ->
     all_fresh src ->
     ws_lang tgt ->
     (forall c t,
         wf_sort src c t ->
         map fst c = map fst s ->
-        compile_sort cmp t[/s/] = (compile_sort cmp t)[/compile_subst cmp s/])
+        forall cname, 
+          In cname cnames ->
+        compile_sort (cnames,cmp) cname t[/s/]
+        = (compile_sort (cnames,cmp) cname t)[/compile_subst (cnames,cmp) s/])
     /\ (forall c e t,
            wf_term src c e t ->
            map fst c = map fst s ->
-           compile cmp e[/s/] = (compile cmp e)[/compile_subst cmp s/])
+        forall cname, 
+          In cname cnames ->
+           compile (cnames,cmp) cname e[/s/]
+           = (compile (cnames,cmp) cname e)[/compile_subst (cnames,cmp) s/])
     /\ (forall c s' c',
            wf_args src c s' c' ->
            map fst c = map fst s ->
-           compile_args cmp s'[/s/] = (compile_args cmp s')[/compile_subst cmp s/]).
+           compile_args (cnames,cmp) s'[/s/]
+           = (compile_args (cnames,cmp) s')[/compile_subst (cnames,cmp) s/]).
 Proof using.
   intros; apply wf_judge_ind; 
     basic_goal_prep;
-    basic_core_crush.
+    basic_core_firstorder_crush.
   {
     case_match; basic_core_crush.
-    case_match; basic_core_firstorder_crush;
-      pose proof (lang_compiler_sort_case_args_eq _ _ _ _ _ H H0 H2 HeqH4);
-      basic_core_firstorder_crush.
+    case_match; auto.
+    replace args0 with (map fst c').
+    unfold env_args.
+    pose proof @compile_args_to_subst.
+    unfold env_args in H8; erewrite !H8.
+    clear H8.
+    rewrite subst_assoc.
+    fold_Substable.
+    rewrite <- with_names_from_args_subst.
+    rewrite H7.
+    reflexivity.
+    rewrite map_fst_with_names_from.
+    pose proof (sort_case_in_preserving_well_scoped _ _ _ H ltac:(basic_core_crush) HeqH8).
+    pose proof (lang_compiler_sort_case_args_eq _ _ _ _ _ H H0 H2 HeqH8).
+    subst.
+    enough (all (fun p => well_scoped (env_args (cnames,[]) (map fst c')) (snd p))
+                (combine cnames tl)).
     {
-      fold_Substable.
-      match goal with
-        [H : compile_args _ _ = _|-_] =>
-        unfold compile_args in H;
-          rewrite H
-      end.
-      erewrite with_names_from_args_subst.
-      reflexivity.
+      eapply P_of_named_list_lookup_from_all_combined in H9.
+      erewrite <- env_args_as_fst_ctx; try reflexivity.
+      exact H9.
+      auto.
+      eapply sort_case_length_in_preserving; eauto.
+    }
+    {
+      revert H8.
+      pose proof (sort_case_length_in_preserving _ _ _ H HeqH8) as H8; revert H8.
+      clear.
+      open_generalize (env_args _ _); intro args.
+      revert tl; induction cnames;
+        destruct tl;
+        basic_goal_prep;
+        basic_core_firstorder_crush.
+    }
+    {
+      unfold compile_ctx, compile_args;
+      erewrite !flat_map_const_len.
+      f_equal.
+      basic_core_crush.
+      all: intros; simpl; try case_match; rewrite ?map_length; reflexivity.
+    }
+    {
+      symmetry; eapply lang_compiler_sort_case_args_eq; eauto.
     }
   }
   {
     case_match; basic_core_crush.
-    case_match; basic_core_firstorder_crush.
-    pose proof (lang_compiler_term_case_args_eq _ _ _ _ _ _ H H0 H2 HeqH4);
-      basic_core_firstorder_crush.
+    case_match; auto.
+    replace args0 with (map fst c').
+    unfold env_args.
+    pose proof @compile_args_to_subst.
+    unfold env_args in H8; erewrite !H8.
+    clear H8.
+    rewrite subst_assoc.
+    fold_Substable.
+    rewrite <- with_names_from_args_subst.
+    all:change (flat_map
+           (fun x : term =>
+            map
+              (fun cname0 : string =>
+                 compile (?cnames, ?cmp) cname0 x) ?cnames))
+      with (compile_args (cnames, cmp)).
+    rewrite !H7.
+    reflexivity.
+    rewrite map_fst_with_names_from.
+    pose proof (term_case_in_preserving_well_scoped _ _ _ H ltac:(basic_core_crush) HeqH8).
+    pose proof (lang_compiler_term_case_args_eq _ _ _ _ _ _ H H0 H2 HeqH8).
+    subst.
+    enough (all (fun p => well_scoped (env_args (cnames,[]) (map fst c')) (snd p))
+                (combine cnames el)).
     {
-      fold_Substable.
-      match goal with
-        [H : compile_args _ _ = _|-_] =>
-        unfold compile_args in H;
-          rewrite H
-      end.
-      erewrite with_names_from_args_subst.
-      reflexivity.
+      eapply P_of_named_list_lookup_from_all_combined in H9.
+      erewrite <- env_args_as_fst_ctx; try reflexivity.
+      exact H9.
+      auto.
+      eapply term_case_length_in_preserving; eauto.
     }
-    pose proof (lang_compiler_term_case_args_eq _ _ _ _ _ _ H H0 H2 HeqH4);
-      basic_core_firstorder_crush.
+    {
+      revert H8.
+      pose proof (term_case_length_in_preserving _ _ _ H HeqH8) as H8; revert H8.
+      clear.
+      open_generalize (env_args _ _); intro args.
+      revert el; induction cnames;
+        destruct el;
+        basic_goal_prep;
+        basic_core_firstorder_crush.
+    }
+    {
+      unfold compile_ctx, compile_args;
+      erewrite !flat_map_const_len.
+      f_equal.
+      basic_core_crush.
+      all: intros; simpl; try case_match; rewrite ?map_length; reflexivity.
+    }
+    {
+      symmetry; eapply lang_compiler_term_case_args_eq; eauto.
+    }
+  }
+  {
+    unfold apply_subst,substable_args, substable_term, args_subst.
+    basic_utils_crush.
+    unfold apply_subst,substable_args, substable_term, args_subst; simpl.
+    fold_Substable.
+    f_equal.
+    {
+      apply map_ext_in; 
+        basic_goal_prep;
+        basic_core_firstorder_crush.
+    }
+    {
+      change (map (term_subst ?s) ?l) with (l[/s/]).
+      assumption.
+    }
   }
 Qed.
 
-Lemma compile_term_subst tgt cmp src s c e t
-  : preserving_compiler_ext [] tgt cmp src ->
+Lemma compile_term_subst tgt cmp src s c e t cnames cname
+  : preserving_compiler_ext (cnames,[]) tgt cmp src ->
     all_fresh src ->
     ws_lang tgt ->
     wf_term src c e t ->
     map fst c = map fst s ->
-    compile cmp e[/s/] = (compile cmp e)[/compile_subst cmp s/].
+    In cname cnames ->
+    compile (cnames,cmp) cname e[/s/]
+    = (compile (cnames,cmp) cname e)[/compile_subst (cnames,cmp) s/].
 Proof.
   intros; eapply distribute_compile_subst; eassumption.
 Qed.
 Hint Rewrite compile_term_subst : lang_core.
 
 
-Lemma compile_sort_subst tgt cmp src s c t
-  : preserving_compiler_ext [] tgt cmp src ->
+Lemma compile_sort_subst tgt cmp src s c t cnames cname
+  : preserving_compiler_ext (cnames,[]) tgt cmp src ->
     all_fresh src ->
     ws_lang tgt ->
     wf_sort src c t ->
     map fst c = map fst s ->
-    compile_sort cmp t[/s/] = (compile_sort cmp t)[/compile_subst cmp s/].
+    In cname cnames ->
+    compile_sort (cnames,cmp) cname t[/s/]
+    = (compile_sort (cnames,cmp) cname t)[/compile_subst (cnames,cmp) s/].
 Proof.
   intros; eapply distribute_compile_subst; eassumption.
 Qed.
 Hint Rewrite compile_sort_subst : lang_core.
 
 
-Lemma compile_args_subst tgt cmp src s c s' c'
-  : preserving_compiler_ext [] tgt cmp src ->
+Lemma compile_args_subst tgt cmp src s c s' c' cnames
+  : preserving_compiler_ext (cnames,[]) tgt cmp src ->
     all_fresh src ->
     ws_lang tgt ->
     wf_args src c s' c' ->
     map fst c = map fst s ->
-    compile_args cmp s'[/s/] = (compile_args cmp s')[/compile_subst cmp s/].
+    compile_args (cnames,cmp) s'[/s/]
+    = (compile_args (cnames,cmp) s')[/compile_subst (cnames,cmp) s/].
 Proof.
   intros; eapply distribute_compile_subst; eassumption.
 Qed.
 Hint Rewrite compile_args_subst : lang_core.
 
+(*
 Lemma compile_subst_with_names_from A cmp (c':named_list A) s
   : (compile_subst cmp (with_names_from c' s)) = with_names_from c' (map (compile cmp) s).
 Proof.
@@ -638,21 +1040,40 @@ Proof.
   rewrite <- with_names_from_map_is_named_map.
   reflexivity.
 Qed.
+*)
 
-Lemma compile_scon cmp args s name t
+Existing Instance sort_default.
+
+
+(* TODO: move generalization to utils*)
+
+Lemma named_list_lookup_none {A}
+      (l : named_list A) (s:list string) (a:A)
+  : None = Utils.named_list_lookup_err l s ->
+    ~ In (s, a) l.
+Proof.
+  induction l; basic_goal_prep; basic_utils_crush.
+  my_case Hs (eqb s l0); basic_goal_prep; basic_utils_crush.
+Qed.
+
+Lemma compile_scon cmp args s name t cname cnames
   : all_fresh cmp ->
     In (name, sort_case args t) cmp ->
-    (compile_sort cmp (scon name s)) = t[/(combine args (compile_args cmp s))/].
+    In cname cnames ->
+    length cnames = length t ->
+    (compile_sort (cnames,cmp) cname (scon name s))
+    = (named_list_lookup default (combine cnames t) cname)
+        [/(combine (env_args (cnames, cmp) args) (compile_args (cnames,cmp) s))/].
 Proof.
   basic_goal_prep; repeat case_match; basic_core_crush.
   {
     (*TODO: should be automated; how best to do so?*)
-    pose proof (in_all_fresh_same _ _ _ _ H H0 HeqH1).
+    pose proof (in_all_fresh_same _ _ _ _ H H0 HeqH3).
     basic_core_crush.
   }
   {
     (*TODO: should be automated; how best to do so?*)
-    pose proof (in_all_fresh_same _ _ _ _ H H0 HeqH1).
+    pose proof (in_all_fresh_same _ _ _ _ H H0 HeqH3).
     basic_core_crush.
   }
   {
@@ -696,15 +1117,86 @@ Proof.
   eauto with utils.
 Qed.
 Hint Resolve lang_compiler_conflict_term_sort : lang_core.
-  
-  
+
+
+Lemma combine_map {A B C D} (f : A -> C) (g : B -> D) l1 l2 
+  : combine (map f l1) (map g l2)
+    = map (fun '(a,b) => (f a,g b)) (combine l1 l2).
+Proof.
+  revert l2; induction l1; destruct l2;
+    basic_goal_prep;
+    basic_utils_crush.
+Qed.
+
+
+Lemma map_combine_XX {A B} (f : A * A -> B) x
+  : map f (combine x x) = map (fun a => f(a,a)) x.
+Proof.
+  induction x; 
+    basic_goal_prep;
+    basic_utils_crush.
+Qed.
+
+Lemma compile_subst_with_names_from cnames cmp c' s
+  : length c' = length s ->
+    (compile_subst (cnames, cmp) (with_names_from c' s))
+    = with_names_from (compile_ctx (cnames, cmp) c')
+                      (compile_args (cnames, cmp) s).
+Proof.
+  revert s; induction c';
+    destruct s;
+    basic_goal_prep;
+    basic_core_crush.
+  rewrite IHc'; auto.
+  f_equal.
+  rewrite <- !combine_map_fst_is_with_names_from.
+  rewrite map_map.
+  simpl.
+  rewrite combine_map.
+  rewrite map_combine_XX.
+  simpl.
+  reflexivity.
+Qed.
+
+
+Lemma compiled_args_len cnames cname cmp c s c' lt
+  : In cname cnames ->
+    wf_args lt (compile_ctx (cnames, cmp) c) (compile_args (cnames, cmp) s) (compile_ctx (cnames, cmp) c') ->
+    Datatypes.length c' = Datatypes.length s.
+Proof.
+  intros inc wfa;
+    apply wf_args_length_eq in wfa;
+    unfold compile_args, compile_ctx in *.
+  enough (length cnames * length c' = length cnames * length s).
+  {
+    revert inc H.
+    clear.
+    intro inc.
+    assert (length cnames > 0) by (destruct cnames; basic_goal_prep; basic_utils_crush; lia).
+    rewrite PeanoNat.Nat.mul_cancel_l; auto; lia.
+  }
+  erewrite !flat_map_const_len in wfa.
+  eassumption.
+  all: intros; simpl; break;
+    rewrite map_length; reflexivity.
+Qed.
+Local Hint Resolve compiled_args_len : core.
+
 (*TODO: do the same thing for terms*)
-Lemma inductive_implies_semantic_sort_rule ls lt cmp name c c' args s
-  : wf_lang lt -> preserving_compiler_ext [] lt cmp ls -> wf_lang ls ->
+Lemma inductive_implies_semantic_sort_rule
+      ls lt cmp name c c' args s
+      cnames cname
+  : wf_lang lt ->
+    preserving_compiler_ext (cnames,[]) lt cmp ls ->
+    wf_lang ls ->
     In (name, sort_rule c' args) ls ->
-    wf_ctx lt (compile_ctx cmp c') ->
-    wf_args lt (compile_ctx cmp c) (compile_args cmp s) (compile_ctx cmp c') ->
-    wf_sort lt (compile_ctx cmp c) (compile_sort cmp (scon name s)).
+    In cname cnames ->
+    wf_ctx lt (compile_ctx (cnames,cmp) c') ->
+    wf_args lt (compile_ctx (cnames,cmp) c)
+            (compile_args (cnames,cmp) s)
+            (compile_ctx (cnames,cmp) c') ->
+    wf_sort lt (compile_ctx (cnames,cmp) c)
+            (compile_sort (cnames,cmp) cname (scon name s)).
 Proof.
   intros.
   replace (scon name s) with (scon name (id_args c'))[/(with_names_from c' s)/].
@@ -720,33 +1212,29 @@ Proof.
   all: basic_core_firstorder_crush.
   {
     rewrite compile_subst_with_names_from.
-    erewrite <- with_names_from_compile_ctx.
     eapply wf_subst_from_wf_args; basic_core_crush.
-  }
-  {
-    pose proof (wf_args_length_eq H4).
-    unfold compile_args in H5.
-    unfold compile_ctx in H5.
-    basic_core_crush.
+    eapply compiled_args_len; eauto.
   }
   {
     simpl; f_equal.
     rewrite wf_con_id_args_subst; basic_core_firstorder_crush.
-    rewrite <- all_fresh_compile_ctx.
-    eauto with lang_core.
-    pose proof (wf_args_length_eq H4).
-    unfold compile_args in H5.
-    unfold compile_ctx in H5.
+    use_rule_in_wf.
+    inversion H6.
     basic_core_crush.
   }
 Qed.
 
-Lemma inductive_implies_semantic_term_rule ls lt cmp name c c' args t s
-  : wf_lang lt -> preserving_compiler_ext [] lt cmp ls -> wf_lang ls ->
+Lemma inductive_implies_semantic_term_rule cnames ls lt cmp name c c' args t s cname
+  : wf_lang lt ->
+    preserving_compiler_ext (cnames,[]) lt cmp ls ->
+    wf_lang ls ->
     In (name, term_rule c' args t) ls ->
-    wf_ctx lt (compile_ctx cmp c') ->
-    wf_args lt (compile_ctx cmp c) (compile_args cmp s) (compile_ctx cmp c') ->
-    wf_term lt (compile_ctx cmp c) (compile cmp (con name s)) (compile_sort cmp t)[/compile_subst cmp (with_names_from c' s)/].
+    In cname cnames ->
+    wf_ctx lt (compile_ctx (cnames,cmp) c') ->
+    wf_args lt (compile_ctx (cnames,cmp) c) (compile_args (cnames,cmp) s) (compile_ctx (cnames,cmp) c') ->
+    wf_term lt (compile_ctx (cnames,cmp) c)
+            (compile (cnames,cmp) cname (con name s))
+            (compile_sort (cnames,cmp) cname t)[/compile_subst (cnames,cmp) (with_names_from c' s)/].
 Proof.
   intros.
   replace (con name s) with (con name (id_args c'))[/(with_names_from c' s)/].
@@ -759,29 +1247,18 @@ Proof.
   {
     eapply inductive_implies_semantic_term_rule_id; eauto.
   }
-  {
-    basic_core_crush.
-  }
+  all: basic_core_firstorder_crush.
   {
     rewrite compile_subst_with_names_from.
-    erewrite <- with_names_from_compile_ctx.
     eapply wf_subst_from_wf_args; basic_core_crush.
-  }
-  {
-    pose proof (wf_args_length_eq H4).
-    unfold compile_args in H5.
-    unfold compile_ctx in H5.
-    basic_core_firstorder_crush.
+    eapply compiled_args_len; eauto.
   }
   {
     simpl; f_equal.
     fold_Substable.
     rewrite wf_con_id_args_subst; basic_core_firstorder_crush.
-    rewrite <- all_fresh_compile_ctx.
-    eauto with lang_core.
-    pose proof (wf_args_length_eq H4).
-    unfold compile_args in H5.
-    unfold compile_ctx in H5.
+    use_rule_in_wf.
+    inversion H6.
     basic_core_crush.
   }
 Qed.
@@ -795,7 +1272,7 @@ Variant rule_compiles_with {lt cmp} : rule -> Prop :=
   : wf_ctx lt (compile_ctx cmp c) -> rule_compiles_with (sort_rule c args)
 | term_rule_compiles_with c args t
   : wf_ctx lt (compile_ctx cmp c) ->
-    wf_sort lt (compile_ctx cmp c) (compile_sort cmp t) ->
+    (forall cname, In cname (fst cmp) -> wf_sort lt (compile_ctx cmp c) (compile_sort cmp cname t)) ->
     rule_compiles_with (term_rule c args t)
 (*Similar properties are not necessary for eq rules*)
 | sort_eq_rule_compiles_with c t1 t2 : rule_compiles_with (sort_eq_rule c t1 t2)
@@ -838,10 +1315,12 @@ Proof.
 Qed.
 Local Hint Resolve lang_compiles_with_term_ctx_in : lang_core.
 
-Lemma lang_compiles_with_term_sort_in lt cmp ls n c' args t
+
+Lemma lang_compiles_with_term_sort_in lt cmp ls n c' args t cname
   : lang_compiles_with lt cmp ls ->
     In (n, term_rule c' args t) ls ->
-    wf_sort lt (compile_ctx cmp c') (compile_sort cmp t).
+    In cname (fst cmp) ->
+    wf_sort lt (compile_ctx cmp c') (compile_sort cmp cname t).
 Proof.
   induction ls; 
     basic_goal_prep;
@@ -855,12 +1334,21 @@ Qed.
 Local Hint Resolve lang_compiles_with_term_sort_in : lang_core.
 
 
-Local Lemma inductive_implies_semantic' lt cmp ls
+
+Lemma in_flat_map {A B} x (f : A -> list B) l a
+  : In x l -> In a (f x) -> In a (flat_map f l).
+Proof.
+  induction l;
+    basic_goal_prep;
+    basic_utils_firstorder_crush.
+Qed.
+
+Local Lemma inductive_implies_semantic' cnames lt cmp ls
   : wf_lang ls ->
     wf_lang lt ->
-    preserving_compiler_ext [] lt cmp ls ->
-    lang_compiles_with lt cmp ls ->
-    semantics_preserving lt cmp ls.
+    preserving_compiler_ext (cnames,[]) lt cmp ls ->
+    lang_compiles_with lt (cnames,cmp) ls ->
+    semantics_preserving lt (cnames,cmp) ls.
 Proof.
   intros; apply judge_ind; 
     basic_goal_prep;
@@ -889,17 +1377,8 @@ Proof.
     eapply inductive_implies_semantic_term_axiom; eassumption.
   }
   {
-    constructor; basic_core_firstorder_crush.
-    match goal with
-      [ H : eq_term _ _ (compile_sort _ _) _ _|-_] =>
-      erewrite !compile_sort_subst in H
-    end.
-    all: try match goal with
-               [|- map fst _ = map fst _] =>
-               symmetry; eauto with lang_core
-             end.
-    all: basic_core_firstorder_crush.
-  }
+    admit (*TODO: eq_subst app/induction on cnames?*).
+  } 
   {
     eapply inductive_implies_semantic_sort_rule; try eassumption.
     all: try use_rule_in_wf; basic_core_firstorder_crush.
@@ -917,34 +1396,25 @@ Proof.
   }
   {
     constructor.
-    apply in_named_map; assumption.
+    unfold compile_ctx.
+    eapply in_flat_map; eauto.
+    simpl.
+    rewrite in_map_iff; eauto.
   }
   {
-    constructor; basic_core_firstorder_crush.
-    match goal with
-      [ H : wf_term _ _ _ (compile_sort _ _) |-_] =>
-      erewrite !compile_sort_subst in H
-    end.
-    all: try match goal with
-               [|- map fst _ = map fst _] =>
-               symmetry; eauto with lang_core
-             end.
-    all: basic_core_firstorder_crush.
-    match goal with
-      [H : context [compile_subst _ (with_names_from _ _)]|-_] =>
-      rewrite compile_subst_with_names_from in H
-    end.
-    rewrite with_names_from_compile_ctx.
-    assumption.
+    admit (*wf_args app*).
   }
-Qed.
+  {
+    admit (*wf_ctx app*).
+  }
+Admitted.
 
-Local Lemma inductive_implies_semantic_ctx' lt cmp ls
+Local Lemma inductive_implies_semantic_ctx' lt cmp ls cnames
   : wf_lang ls ->
     wf_lang lt ->
-    preserving_compiler_ext [] lt cmp ls ->
-    lang_compiles_with lt cmp ls ->
-    forall c : ctx, wf_ctx ls c -> wf_ctx lt (compile_ctx cmp c).
+    preserving_compiler_ext (cnames,[]) lt cmp ls ->
+    lang_compiles_with lt (cnames,cmp) ls ->
+    forall c : ctx, wf_ctx ls c -> wf_ctx lt (compile_ctx (cnames,cmp) c).
 Proof.
   intros wfs wft pc lcw.
   apply inductive_implies_semantic'; eauto.
@@ -954,34 +1424,28 @@ Local Hint Resolve inductive_implies_semantic_ctx' : lang_core.
 
 Local Hint Constructors rule_compiles_with : lang_core.
 
-Definition all_constructors_rule P r :=
-  match r with
-  | sort_rule c _ => all (fun '(_, t) => all_constructors_sort P t) c
-  | term_rule c _ t =>
-    (all (fun '(_, t) => all_constructors_sort P t) c)
-    /\ (all_constructors_sort P t)
-  | _ => True
-  end.
-
-Local Lemma rule_compiles_extend_fresh lt cmp r n cc
-  : rule_compiles_with lt cmp r ->
-    all_constructors_rule (fun n0 : V => In n0 (map fst cmp)) r ->
+Local Lemma rule_compiles_extend_fresh lt cmp r n cc cnames
+  : rule_compiles_with lt (cnames,cmp) r ->
+    all_constructors_rule (fun n0 => In n0 (map fst cmp)) r ->
     fresh n cmp ->
     all_fresh cmp ->
-    rule_compiles_with lt ((n,cc)::cmp) r.
+    rule_compiles_with lt (cnames,(n,cc)::cmp) r.
 Proof.
   inversion 1; basic_goal_prep; with_rule_in_wf_crush.
   all: constructor.
   all: try erewrite compile_strengthen_ctx; eauto.
-  all: try rewrite compile_strengthen_sort; eauto.
+  {
+    intros.
+    erewrite compile_strengthen_sort;eauto.
+  }    
 Qed. 
   
-Local Lemma lang_compiles_extend_fresh lt cmp ls n cc
-  : lang_compiles_with lt cmp ls ->
-    all (fun '(_,r) => all_constructors_rule (fun n0 : V => In n0 (map fst cmp)) r) ls ->
+Local Lemma lang_compiles_extend_fresh lt cmp ls n cc cnames
+  : lang_compiles_with lt (cnames,cmp) ls ->
+    all (fun '(_,r) => all_constructors_rule (fun n0 => In n0 (map fst cmp)) r) ls ->
     fresh n cmp ->
     all_fresh cmp ->
-    lang_compiles_with lt ((n,cc)::cmp) ls.
+    lang_compiles_with lt (cnames,(n,cc)::cmp) ls.
 Proof.
   unfold lang_compiles_with.
   induction ls; basic_goal_prep; with_rule_in_wf_crush.
@@ -989,10 +1453,10 @@ Proof.
 Qed.  
 
 (*TODO: move to core with like lemmas above*)
-Lemma all_constructors_rule_from_wf tgt cmp src r
-  : preserving_compiler_ext [] tgt cmp src ->
+Lemma all_constructors_rule_from_wf tgt cmp src r cnames
+  : preserving_compiler_ext (cnames,[]) tgt cmp src ->
     wf_rule src r ->
-    all_constructors_rule (fun n0 : V => In n0 (map fst cmp)) r.
+    all_constructors_rule (fun n0 => In n0 (map fst cmp)) r.
 Proof.
   inversion 2; basic_goal_prep;
     with_rule_in_wf_crush.
@@ -1001,87 +1465,19 @@ Proof.
 Qed.
 Hint Resolve all_constructors_rule_from_wf : lang_core.
 
-Lemma all_constructors_term_weaken (P Q : _ -> Prop) e
-  : (forall n, P n -> Q n) ->
-    all_constructors P e ->
-    all_constructors Q e.
-Proof.
-  intro.
-  induction e; basic_goal_prep; basic_core_firstorder_crush.
-
-  revert dependent l;
-    induction l; basic_goal_prep; basic_core_crush.
-Qed.
-Hint Resolve all_constructors_term_weaken : lang_core.
-
-
-Lemma all_constructors_args_weaken (P Q : _ -> Prop) l
-  : (forall n, P n -> Q n) ->
-    all (all_constructors P) l ->
-    all (all_constructors Q) l.
-Proof.
-  intro;
-    revert dependent l;
-    induction l; basic_goal_prep; basic_core_crush.
-Qed.
-Hint Resolve all_constructors_args_weaken : lang_core.
-
-
-Lemma all_constructors_sort_weaken (P Q : _ -> Prop) e
-  : (forall n, P n -> Q n) ->
-    all_constructors_sort P e ->
-    all_constructors_sort Q e.
-Proof.
-  intro.
-  destruct e; basic_goal_prep; basic_core_crush.
-Qed.
-Hint Resolve all_constructors_sort_weaken : lang_core.
-
-Lemma all_constructors_ctx_weaken (P Q : _ -> Prop) (c : ctx)
-  : (forall n, P n -> Q n) ->
-    all_constructors_ctx P c ->
-    all_constructors_ctx Q c.
-Proof.
-  intro;
-    induction c; basic_goal_prep; basic_core_crush.
-Qed.
-Hint Resolve all_constructors_ctx_weaken : lang_core.
-
-
-Lemma all_constructors_rule_weaken (P Q : _ -> Prop) r
-  : (forall n, P n -> Q n) ->
-    all_constructors_rule P r ->
-    all_constructors_rule Q r.
-Proof.
-  intro;
-    destruct r; basic_goal_prep; basic_core_crush.
-  all: eapply all_constructors_ctx_weaken; eauto.
-Qed.
-Hint Resolve all_constructors_rule_weaken : lang_core.
-
-
-Lemma all_constructors_lang_weaken (P Q : _ -> Prop) (l : lang)
-  : (forall n, P n -> Q n) ->
-    all (fun '(_, t) => all_constructors_rule P t) l ->
-    all (fun '(_, t) => all_constructors_rule Q t) l.
-Proof.
-  intro;
-    induction l; basic_goal_prep; basic_core_crush.
-Qed.
-Hint Resolve all_constructors_lang_weaken : lang_core.
 
 Lemma wf_lang_implies_all_constructors lt l
   : wf_lang l ->
-    forall cmp,
-    preserving_compiler_ext [] lt cmp l ->
-    all (fun '(_,r) => all_constructors_rule (fun n0 : V => In n0 (map fst cmp)) r) l.
+    forall cnames cmp,
+    preserving_compiler_ext (cnames,[]) lt cmp l ->
+    all (fun '(_,r) => all_constructors_rule (fun n0 => In n0 (map fst cmp)) r) l.
 Proof.
   induction 1; basic_goal_prep;
     with_rule_in_wf_crush.
   (*TODO: break down cmp*)
   inversion H2; subst.
-  1,2:specialize (IHwf_lang_ext cmp0).
-  3,4:specialize (IHwf_lang_ext cmp).
+  1,2:specialize (IHwf_lang_ext cnames cmp0).
+  3,4:specialize (IHwf_lang_ext cnames cmp).
   all:eapply all_constructors_lang_weaken.
   all: try apply IHwf_lang_ext; auto.
   all:basic_goal_prep; basic_core_firstorder_crush.
@@ -1091,31 +1487,36 @@ Qed.
 Local Lemma preserving_compiler_to_lang_compiles_with lt ls
   : wf_lang ls ->
     wf_lang lt ->
-    forall cmp,
-    preserving_compiler_ext [] lt cmp ls ->
-    lang_compiles_with lt cmp ls.
+    forall cnames cmp,
+    preserving_compiler_ext (cnames,[]) lt cmp ls ->
+    lang_compiles_with lt (cnames,cmp) ls.
 Proof.
-  induction 1; inversion 2; basic_goal_prep; with_rule_in_wf_crush.
+  induction 1; inversion 2; basic_goal_prep; try use_rule_in_wf; basic_core_firstorder_crush.
   all: try constructor.
   all: try rewrite compile_strengthen_ctx; eauto.
-  all: try rewrite compile_strengthen_sort; eauto.
+  all: try (intros; rewrite compile_strengthen_sort; eauto).
   all: try apply lang_compiles_extend_fresh; eauto with lang_core.
   all: try eapply wf_lang_implies_all_constructors; eauto.
-  all: eapply all_constructors_ctx_from_wf; [| eauto..]; eauto.
+  {
+    simpl in *.
+     (*TODO: hack for missing lemma*)
+    eapply eq_term_wf_sort; auto;
+      [basic_core_firstorder_crush
+      | eapply eq_term_refl; auto].
+    unshelve(eapply P_of_named_list_lookup_from_all_combined in H9); eauto; exact (con [] []).
+  }
 Qed.
 
 
-Theorem inductive_implies_semantic lt cmp ls
+Theorem inductive_implies_semantic lt cmp ls cnames
   : wf_lang ls ->
     wf_lang lt ->
-    preserving_compiler_ext [] lt cmp ls ->
-    semantics_preserving lt cmp ls.
+    preserving_compiler_ext (cnames,[]) lt cmp ls ->
+    semantics_preserving lt (cnames,cmp) ls.
 Proof.
   intros; apply inductive_implies_semantic';
-    eauto using  preserving_compiler_to_lang_compiles_with.
+    eauto using preserving_compiler_to_lang_compiles_with.
 Qed.
-
-End WithVar.
 
 
 #[export] Hint Rewrite fresh_compile_ctx : lang_core.
@@ -1150,9 +1551,3 @@ End WithVar.
 
 
 #[export] Hint Resolve all_constructors_rule_from_wf : lang_core.
-#[export] Hint Resolve all_constructors_term_weaken : lang_core.
-#[export] Hint Resolve all_constructors_args_weaken : lang_core.
-#[export] Hint Resolve all_constructors_sort_weaken : lang_core.
-#[export] Hint Resolve all_constructors_ctx_weaken : lang_core.
-#[export] Hint Resolve all_constructors_rule_weaken : lang_core.
-#[export] Hint Resolve all_constructors_lang_weaken : lang_core.
